Regex/Termination.lean
@@ -1,10 +1,77 @@
-import Regex.Basic
+import Regex.Lemmas.Bounds
 
 namespace Regex
 
 variable {α : Type u} [deq : DecidableEq α] {r : Regex α} {w : List α}
 
-/-- A class of regexes that can be proven to terminate -/
+section Tactic
+
+open Lean Parser Tactic
+
+macro "termination" : tactic =>
+  `(tactic| (repeat simp [
+    terminates_bot, terminates_empty, terminates_unit, terminates_concat,
+    terminates_or, terminates_filterEmpty, terminates_start, terminates_end',
+    terminates_capture, terminates_backref, terminates_star_of_forall];
+    ))
+
+end Tactic
+
+/-- A regex that always terminates, regardless of inputs to `matchPartial` -/
+def AlwaysTerminates (r : Regex α) := ∀ w s cap, r.Terminates w s cap
+
+theorem alwaysTerminates_bot : [/⊥/].AlwaysTerminates (α := α) :=
+  fun _ _ _ ↦ terminates_bot
+
+theorem alwaysTerminates_empty : [//].AlwaysTerminates (α := α) :=
+  fun _ _ _ ↦ terminates_empty
+
+theorem alwaysTerminates_unit {c : α} : [/c/].AlwaysTerminates (α := α) :=
+  fun _ _ _ ↦ terminates_unit
+
+theorem alwaysTerminates_concat {q r : Regex α}
+    (qt : q.AlwaysTerminates) (rt : r.AlwaysTerminates)
+    : [/⟨q⟩ ⟨r⟩/].AlwaysTerminates (α := α) :=
+  fun w s cap ↦ terminates_concat.mpr ⟨qt w s cap, fun mat _ ↦ rt w mat.1 mat.2⟩
+
+theorem alwaysTerminates_or {q r : Regex α}
+    (qt : q.AlwaysTerminates) (rt : r.AlwaysTerminates)
+    : [/⟨q⟩ | ⟨r⟩/].AlwaysTerminates (α := α) :=
+  fun w s cap ↦ terminates_or.mpr ⟨qt w s cap, rt w s cap⟩
+
+theorem alwaysTerminates_or_comm {q r : Regex α}
+    : [/⟨q⟩ | ⟨r⟩/].AlwaysTerminates ↔ [/⟨r⟩ | ⟨q⟩/].AlwaysTerminates := by
+  simp only [AlwaysTerminates, terminates_or_comm (q := q)]
+
+theorem alwaysTerminates_filterEmpty {e : Bool} {r : Regex α}
+    (rt : r.AlwaysTerminates)
+    : [/⟨r⟩ ‹e›ε/].AlwaysTerminates (α := α) :=
+  fun w s cap ↦ terminates_filterEmpty.mpr (rt w s cap)
+
+theorem alwaysTerminates_star {t : StarType} {r : Regex α}
+    (rt : r.AlwaysTerminates)
+    : [/⟨r⟩*‹t›/].AlwaysTerminates (α := α) :=
+  fun w _ _ ↦ terminates_star_of_forall fun s' _ cap' ↦ rt w s' cap'
+
+theorem alwaysTerminates_star_greedy_iff_lazy {r : Regex α}
+    : [/⟨r⟩*/].AlwaysTerminates ↔ [/⟨r⟩*?/].AlwaysTerminates := by
+  simp only [AlwaysTerminates, terminates_star_greedy_iff_lazy]
+
+theorem alwaysTerminates_start : [/⊢/].AlwaysTerminates (α := α) :=
+  fun _ _ _ ↦ terminates_start
+
+theorem alwaysTerminates_end' : [/⊣/].AlwaysTerminates (α := α) :=
+  fun _ _ _ ↦ terminates_end'
+
+theorem alwaysTerminates_capture {n : ℕ} {r : Regex α}
+    (rt : r.AlwaysTerminates)
+    : [/(‹n› ⟨r⟩)/].AlwaysTerminates (α := α) :=
+  fun w s cap ↦ terminates_capture.mpr (rt w s cap)
+
+theorem alwaysTerminates_backref {d : BackrefDefault} {n : ℕ}
+    : [/\‹d›n/].AlwaysTerminates (α := α) := fun _ _ _ ↦ terminates_backref
+
+/-- A class of regexes that can be proven to always terminate -/
 inductive classTerminates : Regex α → Prop where
   | bot : classTerminates bot
   | empty : classTerminates empty
@@ -19,19 +86,20 @@ inductive classTerminates : Regex α → Prop where
   | backref d n : classTerminates (backref d n)
 
 /-- Rexeges constructed out of just ones in `classTerminates` always terminate -/
-theorem classTerminates_terminates (r : Regex α) (hr : r.classTerminates)
-    : ∀ w s cap, r.Terminates w s cap := by
+theorem alwaysTerminates_classTerminates {r : Regex α} (hr : r.classTerminates)
+    : r.AlwaysTerminates := by
+  dsimp [AlwaysTerminates]
   induction hr with
   | bot => termination
   | empty => termination
   | unit c => termination
-  | concat q r _ _ qt rt => simp [concat_terminates, qt, rt]
-  | or q r _ _ qt rt => simp [or_terminates, qt, rt]
-  | filterEmpty e r _ rt => simp [filterEmpty_terminates, rt]
-  | star t r _ rt => intro r s cap; apply star_terminates_of_forall; simp [rt]
+  | concat q r _ _ qt rt => simp [terminates_concat, qt, rt]
+  | or q r _ _ qt rt => simp [terminates_or, qt, rt]
+  | filterEmpty e r _ rt => simp [terminates_filterEmpty, rt]
+  | star t r _ rt => intro r s cap; apply terminates_star_of_forall; simp [rt]
   | start => termination
   | end' => termination
-  | capture n r _ rt => simp [capture_terminates, rt]
+  | capture n r _ rt => simp [terminates_capture, rt]
   | backref d n => termination
 
 end Regex
