Regex/Match.lean
@@ -1,0 +1,172 @@
+import Regex.Basic
+
+namespace Regex
+variable {α : Type u} [deq : DecidableEq α] {r : Regex α} {w : List α}
+
+/-! Stuff about full matches -/
+
+/-- Returns all matches that end at the end of the string -/
+def match' (r : Regex α) (w : List α) (term : r.Terminates w 0 0) :
+  PartialMatches := [/⟨r⟩ ⊣/].matchPartial w 0 0
+    (terminates_concat.mpr ⟨term, fun _ _ ↦ terminates_end'⟩)
+
+theorem match'_def (term : r.Terminates w 0 0)
+    : r.match' w term = (r.matchPartial w 0 0 term).filter fun mat ↦ mat.1 = w.length := by
+  rw [match', matchPartial_concat]
+  simp only [matchPartial_end', Prod.mk.eta, List.pmap_eq_map]
+  rw [← List.flatMap_def, ← List.filterMap_eq_filter, List.filterMap_eq_flatMap_toList]
+  simp only [Option.guard_apply, decide_eq_true_eq]
+  congr; ext mat n mat'
+  split <;> simp
+
+theorem mem_match'_iff (term : r.Terminates w 0 0) {mat}
+    : mat ∈ r.match' w term ↔
+      mat ∈ r.matchPartial w 0 0 term ∧ mat.1 = w.length := by simp [match'_def]
+
+/-- The condition specialized for (w.length, cap) -/
+theorem mem_match'_iff_length_mem (term : r.Terminates w 0 0) {cap}
+    : (w.length, cap) ∈ r.match' w term ↔
+      (w.length, cap) ∈ r.matchPartial w 0 0 term := by
+  simp [mem_match'_iff]
+
+/-- Returns whether the whole sequence matches the regex.
+We require termination, because weird properties result without that requirement.
+(e.g. `q.isMatch w` but not `(or q r).isMatch w` because `r` doesn't terminate) -/
+def IsMatch (r : Regex α) (w : List α) (term : r.Terminates w 0 0) :=
+  r.match' w term ≠ []
+
+/-- `⊥` never matches -/
+theorem isMatch_bot : ¬[/⊥/].IsMatch w terminates_bot := by
+  simp [IsMatch, match'_def, matchPartial_bot]
+
+/-- The empty regex matches only the empty string -/
+theorem isMatch_empty : [//].IsMatch w terminates_empty ↔ w = [] := by
+  simp only [IsMatch, match'_def, matchPartial_empty, ne_eq, List.filter_eq_nil_iff, List.mem_cons,
+    List.not_mem_nil, or_false, decide_eq_true_eq, forall_eq, Decidable.not_not]
+  rw [eq_comm, List.length_eq_zero_iff]
+
+/-- A unit regex matches only the singleton sequence that has that unit -/
+theorem isMatch_unit {c : α} : [/`‹c›/].IsMatch w terminates_unit ↔ w = [c] := by
+  simp only [IsMatch, match'_def, matchPartial_unit, zero_add, ne_eq, List.filter_eq_nil_iff,
+    List.mem_ite_nil_right, List.mem_cons, List.not_mem_nil, or_false, decide_eq_true_eq, and_imp,
+    forall_eq_apply_imp_iff, Classical.not_imp, Decidable.not_not]
+  rw [eq_comm (a := 1), List.length_eq_one_iff, List.getElem?_eq_some_iff]
+  constructor
+  · rintro ⟨⟨lt, eqc⟩, ⟨c', eqc'⟩⟩
+    simp only [eqc', List.getElem_cons_zero, List.cons.injEq, and_true] at eqc ⊢
+    exact eqc
+  · intro wc; simp [wc]
+
+theorem isMatch_concat {q r : Regex α} (term : [/⟨q⟩ ⟨r⟩/].Terminates w 0 0)
+    : [/⟨q⟩ ⟨r⟩/].IsMatch w term ↔
+      ∃ mat,
+        ∃ (mem : mat ∈ q.matchPartial w 0 0 (terminates_concat.mp term).1),
+        ∃ mat' ∈ r.matchPartial w mat.1 mat.2
+          ((terminates_concat.mp term).2 _ mem), mat'.1 = w.length := by
+  simp [IsMatch, match'_def, matchPartial_concat]
+
+/-- An alternation between `q` and `r` matches iff `q` matches or `r` matches -/
+theorem isMatch_or {q r : Regex α} (term : [/⟨q⟩ | ⟨r⟩/].Terminates w 0 0)
+    : [/⟨q⟩ | ⟨r⟩/].IsMatch w term ↔
+      q.IsMatch w (terminates_or.mp term).1 ∨ r.IsMatch w (terminates_or.mp term).2 := by
+  simp [IsMatch, match'_def, matchPartial_or, imp_iff_not_or]
+
+theorem decide_eq_bool {p : Prop} [Decidable p] {b : Bool}
+    : decide p = b ↔ (p ↔ b = true) := by cases b <;> simp
+
+theorem isMatch_filterEmpty {e : Bool} {r : Regex α}
+    (term : [/⟨r⟩ ‹e›ε/].Terminates w 0 0)
+    : [/⟨r⟩ ‹e›ε/].IsMatch w term ↔
+      r.IsMatch w (terminates_filterEmpty.mp term) ∧ (w.length = 0) = e := by
+  simp [IsMatch, match'_def, matchPartial_filterEmpty, decide_eq_bool]
+
+-- Some silly ones
+
+/-- The start anchor full-matches only the empty sequence -/
+theorem isMatch_start : [/⊢/].IsMatch w terminates_start ↔ w = [] := by
+  simp only [IsMatch, match'_def, matchPartial_start, ↓reduceIte, ne_eq, List.filter_eq_nil_iff,
+    List.mem_cons, List.not_mem_nil, or_false, decide_eq_true_eq, forall_eq, Decidable.not_not]
+  rw [eq_comm, List.length_eq_zero_iff]
+
+/-- The end anchor full-matches only the empty sequence -/
+theorem isMatch_end' : [/⊣/].IsMatch w terminates_end' ↔ w = [] := by
+  simp only [IsMatch, match'_def, matchPartial_end', ne_eq, List.filter_eq_nil_iff,
+    List.mem_ite_nil_right, List.mem_cons, List.not_mem_nil, or_false, decide_eq_true_eq, and_imp,
+    forall_eq_apply_imp_iff, imp_not_self, Decidable.not_not]
+  rw [eq_comm, List.length_eq_zero_iff]
+
+/-- A capture of `r` matches iff `r` matches -/
+theorem isMatch_capture {n : ℕ} {r : Regex α} (term : [/(‹n› ⟨r⟩)/].Terminates w 0 0)
+    : [/(‹n› ⟨r⟩)/].IsMatch w term ↔ r.IsMatch w (terminates_capture.mp term) := by
+  simp [IsMatch, match'_def, matchPartial_capture]
+
+/-- A full-match on a backref just defaults -/
+theorem isMatch_backref {d : BackrefDefault} {n : ℕ}
+    : [/\‹d›n/].IsMatch w terminates_backref ↔ match d with
+        | .bot => False
+        | .empty => w = [] := by
+  simp [IsMatch, match'_def, matchPartial_backref]
+  split <;> simp
+
+/-- The language of a regex is the set of languages that it full-matches. -/
+def language (r : Regex α) (term : ∀ w, r.Terminates w 0 0)
+  : Language α := {w | IsMatch r w (term w)}
+
+theorem mem_language_iff {r : Regex α} {term : ∀ w, r.Terminates w 0 0} {w}
+    : w ∈ r.language term ↔ r.IsMatch w (term w) := by
+  simp [language]; rfl
+
+theorem language_bot : ([/⊥/] : Regex α).language (fun _ ↦ terminates_bot) = 0 := by
+  simp [language, isMatch_bot]; rfl
+
+theorem language_empty : ([//] : Regex α).language (fun _ ↦ terminates_empty) = {[]} := by
+  simp [language, isMatch_empty]
+
+theorem language_unit {c : α} : [/c/].language (fun _ ↦ terminates_unit) = {[c]} := by
+  simp [language, isMatch_unit]
+
+/-- Not a simple language description, but this is the language of a concat.
+Note that it is *not* the concatenation of the individual languages. -/
+theorem language_concat {q r : Regex α} (term : ∀ w, [/⟨q⟩ ⟨r⟩/].Terminates w 0 0)
+    : [/⟨q⟩ ⟨r⟩/].language term
+      = {w | ∃ mat,
+        ∃ (mem : mat ∈ q.matchPartial w 0 0 (terminates_concat.mp (term w)).1),
+        ∃ mat' ∈ r.matchPartial w mat.1 mat.2
+          ((terminates_concat.mp (term w)).2 _ mem), mat'.1 = w.length} := by
+  simp [language, isMatch_concat]
+
+theorem language_or {q r : Regex α} (term : ∀ w, [/⟨q⟩ | ⟨r⟩/].Terminates w 0 0)
+  : [/⟨q⟩ | ⟨r⟩/].language term
+    = q.language (fun _ ↦ (terminates_or.mp (term _)).1) +
+      r.language (fun _ ↦ (terminates_or.mp (term _)).2) := by
+  simp [language, isMatch_or, Language.add_def, Set.union_def]
+
+theorem language_filterEmpty {e : Bool} {r : Regex α}
+    (term : ∀ w, [/⟨r⟩ ‹e›ε/].Terminates w 0 0)
+    : ([/⟨r⟩ ‹e›ε/] : Regex α).language term = if e then
+        r.language (fun _ ↦ terminates_filterEmpty.mp (term _)) ⊓ {[]} else
+        r.language (fun _ ↦ terminates_filterEmpty.mp (term _)) - {[]} := by
+  simp only [language, isMatch_filterEmpty, List.length_eq_zero_iff, eq_iff_iff]
+  split <;> (expose_names; simp only [h, iff_true, Bool.false_eq_true, iff_false])
+  · ext x; rw [Language.mem_inf, Set.setOf_and, Set.mem_inter_iff]; rfl
+  · ext x; rw [Language.mem_sub, Set.setOf_and, Set.mem_inter_iff]; rfl
+
+theorem language_start : ([/⊢/] : Regex α).language (fun _ ↦ terminates_start) = {[]} := by
+  simp [language, isMatch_start]
+
+theorem language_end' : ([/⊣/] : Regex α).language (fun _ ↦ terminates_end') = {[]} := by
+  simp [language, isMatch_end']
+
+theorem language_capture {n : ℕ} {r : Regex α} (term : ∀ w, [/(‹n› ⟨r⟩)/].Terminates w 0 0)
+    : ([/(‹n› ⟨r⟩)/] : Regex α).language term =
+      r.language (fun _ ↦ terminates_capture.mp (term _)) := by
+  simp [language, isMatch_capture]
+
+theorem language_backref {d : BackrefDefault} {n : ℕ}
+    : ([/\‹d›n/] : Regex α).language (fun _ ↦ terminates_backref) = match d with
+      | .bot => 0
+      | .empty => {[]} := by
+  simp [language, isMatch_backref]
+  split <;> simp; rfl
+
+end Regex
